

Problem 4.4.3(b): Consider a slightly damped vibrating string that satisfies

$$\rho_0 \frac{\partial^2 u}{\partial t^2} = T_0 \frac{\partial^2 u}{\partial x^2} - \beta \frac{\partial u}{\partial t}.$$

Determine the solution (by separation of variables) for a string with fixed ends and with initial conditions $u(x, 0) = f(x)$ and $\frac{\partial u}{\partial t}(x, 0) = g(x)$

First, assume that the solution is separable.

$$u(x, t) = T(t)X(x).$$

Then

$$\rho_0 T'' X = T_0 X'' T - \beta T' X$$

implies

$$\frac{\rho_0 T'' + \beta T'}{T_0 T} = -\lambda = \frac{X''}{X}.$$

First, to find $X(x)$, let $m = \pm\sqrt{\lambda}$. Then

$$X(x) = \sum_{n=1}^{\infty} a_n \sin\left(\frac{n\pi x}{L}\right)$$

and, in the only non-trivial case, $\lambda > 0$,

$$\lambda = \left(\frac{n\pi}{L}\right)^2.$$

Then to find $T(t)$, since

$$\rho_0 T'' + \beta T' + T_0 \lambda T = 0,$$

then

$$\rho_0 m^2 + \beta m + T_0 \lambda = 0$$

and we can solve for m with the quadratic formula,

$$m = \frac{-\beta \pm \sqrt{\beta^2 - 4\rho_0 T_0 \lambda}}{2\rho_0}.$$

Assume that the discriminant is less than zero and let $H = |\beta^2 - 4\rho_0 T_0 \lambda|$. Then,

$$m = \frac{-\beta \pm i\sqrt{H}}{2\rho_0}$$

implies

$$T(t) = e^{-\frac{\beta}{2\rho_0}t} \left(\cos\left(\frac{\sqrt{H}}{2\rho_0}t\right) + \sin\left(\frac{\sqrt{H}}{2\rho_0}t\right) \right).$$

Then,

$$u(x, t) = \sum_{n=1}^{\infty} \sin\left(\frac{n\pi x}{L}\right) e^{-\frac{\beta}{2\rho_0}t} \left(A_n \cos\left(\frac{\sqrt{H}}{2\rho_0}t\right) + B_n \sin\left(\frac{\sqrt{H}}{2\rho_0}t\right) \right)$$

where

$$A_n = \frac{2}{L} \int_0^L f(x) \sin\left(\frac{n\pi x}{L}\right) dx.$$

To get B_n , we differentiate u with respect to t , and apply boundary conditions as follows.

$$\frac{\partial u}{\partial t} = \sum_{n=1}^{\infty} \left(\frac{-\beta}{2\rho_0} e^{-\frac{\beta}{2\rho_0}t} \sin\left(\frac{n\pi x}{L}\right) \right) \left(A_n \cos\left(\frac{\sqrt{H}}{2\rho_0}t\right) + B_n \sin\left(\frac{\sqrt{H}}{2\rho_0}t\right) \right) + \left(e^{-\frac{\beta}{2\rho_0}t} \sin\left(\frac{n\pi x}{L}\right) \right) \left(\frac{\sqrt{H}}{2\rho_0} (B_n \cos\left(\frac{\sqrt{H}}{2\rho_0}t\right) - A_n \sin\left(\frac{\sqrt{H}}{2\rho_0}t\right)) \right)$$

Evaluating this at $t = 0$,

$$g(x) = \sum_{n=1}^{\infty} \left[-A_n \frac{\beta}{2\rho_0} \sin\left(\frac{n\pi x}{L}\right) + B_n \frac{\sqrt{H}}{2\rho_0} \sin\left(\frac{n\pi x}{L}\right) \right]$$

$$g(x) = \sum_{n=1}^{\infty} \left[\left(\frac{-\beta A_n + \sqrt{H} B_n}{2\rho_0} \right) \sin\left(\frac{n\pi x}{L}\right) \right]$$

gives

$$\frac{-\beta A_n + \sqrt{H} B_n}{2\rho_0} = \frac{2}{L} \int_0^L g(x) \sin\left(\frac{n\pi x}{L}\right) dx$$

which yields

$$B_n = \frac{4\rho_0}{L\sqrt{H}} \left(\int_0^L g(x) \sin\left(\frac{n\pi x}{L}\right) dx + \beta A_n \right)$$

Problem 4.4.7: If a vibrating string satisfying (4.4.1)-(4.4.3) is initially at rest ($g(x) = 0$), show that

$$u(x, t) = \frac{1}{2} [F(x - ct) + F(x + ct)],$$

where $F(x)$ is the odd-periodic extension of $f(x)$.

The odd periodic extension of $f(x)$ is defined by

$$f(x) \sim F(x) = \sum_{n=1}^{\infty} B_n \sin\left(\frac{n\pi x}{L}\right)$$

where

$$B_n = \frac{2}{L} \int_0^L f(x) \sin\left(\frac{n\pi x}{L}\right) dx.$$

Accordingly,

$$F(x - ct) = \sum_{n=1}^{\infty} B_n \sin\left(\frac{n\pi x}{L} - \frac{n\pi ct}{L}\right) = \sum_{n=1}^{\infty} B_n \left[\sin\left(\frac{n\pi x}{L}\right) \cos\left(\frac{n\pi ct}{L}\right) - \cos\left(\frac{n\pi x}{L}\right) \sin\left(\frac{n\pi ct}{L}\right) \right]$$

and

$$F(x + ct) = \sum_{n=1}^{\infty} B_n \sin\left(\frac{n\pi x}{L} + \frac{n\pi ct}{L}\right) = \sum_{n=1}^{\infty} B_n \left[\sin\left(\frac{n\pi x}{L}\right) \cos\left(\frac{n\pi ct}{L}\right) + \cos\left(\frac{n\pi x}{L}\right) \sin\left(\frac{n\pi ct}{L}\right) \right]$$

Then,

$$\begin{aligned} & \frac{1}{2} [F(x - ct) + F(x + ct)] = \\ &= \frac{1}{2} \left[\sum_{n=1}^{\infty} B_n \left[\sin\left(\frac{n\pi x}{L}\right) \cos\left(\frac{n\pi ct}{L}\right) + \cos\left(\frac{n\pi x}{L}\right) \sin\left(\frac{n\pi ct}{L}\right) \right] + \sum_{n=1}^{\infty} B_n \left[\sin\left(\frac{n\pi x}{L}\right) \cos\left(\frac{n\pi ct}{L}\right) - \cos\left(\frac{n\pi x}{L}\right) \sin\left(\frac{n\pi ct}{L}\right) \right] \right] \\ &= \sum_{n=1}^{\infty} B_n \sin\left(\frac{n\pi x}{L}\right) \cos\left(\frac{n\pi ct}{L}\right) \end{aligned}$$

which is exactly $u(x, t)$ when $g(x) = 0$.